add absence mixed endpoint

fixtures/TypeChecker.ml
@@ -16799,6 +16799,15 @@ let check_env_end2end_direct_receiver_mixed_ready env =
   (||) (negb (check_env_root_shadow_direct_receiver_method_present env))
     (check_env_end2end_direct_receiver_ready env)
 
+(** val check_env_end2end_direct_receiver_absent_mixed_ready :
+    global_env -> bool **)
+
+let check_env_end2end_direct_receiver_absent_mixed_ready env =
+  (||)
+    ((&&) (negb (check_env_root_shadow_direct_receiver_method_present env))
+      (check_env_root_shadow_captured_call_store_safe_summary_absent env))
+    (check_env_end2end_direct_receiver_ready env)
+
 (** val infer_program_env_end2end_strict_exact_closure_direct_receiver :
     global_env -> global_env infer_result **)
 
@@ -16854,6 +16863,25 @@ let infer_program_env_end2end_assoc_direct_receiver_mixed env =
 
 let check_program_env_end2end_assoc_direct_receiver_mixed env =
   match infer_program_env_end2end_assoc_direct_receiver_mixed env with
+  | Infer_ok _ -> true
+  | Infer_err _ -> false
+
+(** val infer_program_env_end2end_assoc_direct_receiver_absent_mixed :
+    global_env -> global_env infer_result **)
+
+let infer_program_env_end2end_assoc_direct_receiver_absent_mixed env =
+  match infer_program_env_end2end_assoc env with
+  | Infer_ok env' ->
+    if check_env_end2end_direct_receiver_absent_mixed_ready env'
+    then Infer_ok env'
+    else Infer_err ErrEndToEndSafetyGateFailed
+  | Infer_err err -> Infer_err err
+
+(** val check_program_env_end2end_assoc_direct_receiver_absent_mixed :
+    global_env -> bool **)
+
+let check_program_env_end2end_assoc_direct_receiver_absent_mixed env =
+  match infer_program_env_end2end_assoc_direct_receiver_absent_mixed env with
   | Infer_ok _ -> true
   | Infer_err _ -> false
 
