fixtures/TypeChecker.mli
@@ -1604,6 +1604,8 @@ val check_env_root_shadow_direct_receiver_method_present : global_env -> bool
 
 val check_env_end2end_direct_receiver_mixed_ready : global_env -> bool
 
+val check_env_end2end_direct_receiver_absent_mixed_ready : global_env -> bool
+
 val infer_program_env_end2end_strict_exact_closure_direct_receiver :
   global_env -> global_env infer_result
 
@@ -1620,6 +1622,12 @@ val infer_program_env_end2end_assoc_direct_receiver_mixed :
   global_env -> global_env infer_result
 
 val check_program_env_end2end_assoc_direct_receiver_mixed : global_env -> bool
+
+val infer_program_env_end2end_assoc_direct_receiver_absent_mixed :
+  global_env -> global_env infer_result
+
+val check_program_env_end2end_assoc_direct_receiver_absent_mixed :
+  global_env -> bool
 
 val infer_program_env_end2end_assoc_strict_exact_closure_direct_receiver_mixed :
   global_env -> global_env infer_result
